src/program_proof/tulip/invariance/cmd.v
@@ -1,0 +1,34 @@
+From Perennial.program_proof.tulip Require Import prelude.
+
+Section lemma.
+  Context `{!tulip_ghostG Σ}.
+
+  Lemma repl_hist_multiwrite_disjoint {γ} ts wrs hists :
+    dom hists ## dom wrs ->
+    ([∗ map] k ↦ hist ∈ hists, own_repl_hist_half γ k hist) -∗
+    ([∗ map] k ↦ hist ∈ multiwrite ts wrs hists, own_repl_hist_half γ k hist).
+  Proof.
+    iIntros (Hdom) "Htpls".
+    iApply (big_sepM_impl_dom_eq with "Htpls"); first apply multiwrite_dom.
+    iIntros "!>" (k h1 h2 Hh1 Hh2) "Hhist".
+    destruct (wrs !! k) as [v |] eqn:Hwrs.
+    { apply elem_of_dom_2 in Hh1. apply elem_of_dom_2 in Hwrs. set_solver. }
+    rewrite /multiwrite lookup_merge Hwrs Hh1 /= in Hh2.
+    by inv Hh2.
+  Qed.
+
+  Lemma repl_ts_release_disjoint {γ} wrs ptsm :
+    dom ptsm ## dom wrs ->
+    ([∗ map] k ↦ pts ∈ ptsm, own_repl_ts_half γ k pts) -∗
+    ([∗ map] k ↦ pts ∈ release wrs ptsm, own_repl_ts_half γ k pts).
+  Proof.
+    iIntros (Hdom) "Hptsm".
+    iApply (big_sepM_impl_dom_eq with "Hptsm"); first apply release_dom.
+    iIntros "!>" (k t1 t2 Ht1 Ht2) "Hpts".
+    destruct (wrs !! k) as [v |] eqn:Hwrs.
+    { apply elem_of_dom_2 in Ht1. apply elem_of_dom_2 in Hwrs. set_solver. }
+    rewrite /release lookup_merge Hwrs Ht1 /= in Ht2.
+    by inv Ht2.
+  Qed.
+
+End lemma.
