src/program_proof/tulip/invariance/learn_abort.v
@@ -1,0 +1,274 @@
+From Perennial.program_proof.tulip Require Import prelude.
+From Perennial.program_proof.tulip.invariance Require Import cmd.
+
+Lemma ext_by_cmtd_inv_learn_abort {repl cmtd kmod} ts :
+  kmod !! O = None ->
+  kmod !! ts = None ->
+  ext_by_cmtd repl cmtd kmod ts ->
+  ext_by_cmtd repl cmtd kmod O.
+Proof.
+  intros Hz Hts Hdiff.
+  rewrite /ext_by_cmtd Hts in Hdiff.
+  rewrite /ext_by_cmtd Hz.
+  destruct Hdiff as (rts & Hext & _).
+  by exists rts.
+Qed.
+
+Section inv.
+  Context `{!tulip_ghostG Σ}.
+
+  Lemma keys_inv_prepared {γ p ts} keys :
+    is_txn_aborted γ ts -∗
+    ([∗ set] key ∈ keys, key_inv_no_tsprep γ key ts) -∗
+    txnsys_inv γ p -∗
+    ([∗ set] key ∈ keys, key_inv_prepared_no_tsprep γ key ts) ∗
+    txnsys_inv γ p.
+  Proof.
+    iIntros "#Habt Hkeys Htxnsys".
+    iApply (big_sepS_impl_res with "Hkeys Htxnsys").
+    iIntros (k Hk) "!> Hkey Htxnsys".
+    do 2 iNamed "Htxnsys".
+    iDestruct (txn_res_lookup with "Hresm Habt") as %Hresm.
+    do 2 iNamed "Hkey".
+    iDestruct (cmtd_kmod_vslice_agree with "Hkmodcs Hkmodc") as %Hkmodc.
+    { apply Hall. }
+    assert (Hnc : kmodc !! ts = None).
+    { subst kmodc. by eapply vslice_resm_to_tmods_aborted. }
+    iAssert (txnsys_inv γ p)%I with "[-Hkmodl Hkmodc Hdbv Hlnrz Hcmtd Hrepl]" as "Htxnsys".
+    { iFrame "∗ # %". }
+    iFrame "∗ # %".
+  Qed.
+
+  Lemma key_inv_learn_abort {γ ts} k :
+    key_inv_prepared_no_tsprep γ k ts -∗
+    key_inv_no_tsprep γ k O.
+  Proof.
+    iIntros "Hkey".
+    do 3 iNamed "Hkey".
+    iFrame "∗ # %".
+    iPureIntro.
+    by apply (ext_by_cmtd_inv_learn_abort ts).
+  Qed.
+
+  Lemma keys_inv_learn_abort {γ ts keys} :
+    ([∗ set] key ∈ keys, key_inv_prepared_no_tsprep γ key ts) -∗
+    ([∗ set] key ∈ keys, key_inv_no_tsprep γ key O).
+  Proof.
+    iIntros "Hkeys".
+    iApply (big_sepS_mono with "Hkeys").
+    iIntros (k Hk) "Hkey".
+    iApply (key_inv_learn_abort with "Hkey").
+  Qed.
+
+  Lemma group_inv_learn_abort γ p gid log cpool ts :
+    cpool_subsume_log cpool (log ++ [CmdAbort ts]) ->
+    txnsys_inv γ p -∗
+    ([∗ set] key ∈ keys_all, key_inv γ key) -∗
+    group_inv_no_log_with_cpool γ gid log cpool ==∗
+    txnsys_inv γ p ∗
+    ([∗ set] key ∈ keys_all, key_inv γ key) ∗
+    group_inv_no_log_with_cpool γ gid (log ++ [CmdAbort ts]) cpool.
+  Proof.
+    iIntros (Hsubsume) "Htxnsys Hkeys Hgroup".
+    rewrite /cpool_subsume_log Forall_app Forall_singleton in Hsubsume.
+    destruct Hsubsume as [Hsubsume Hc].
+    do 2 iNamed "Hgroup".
+    (* Obtain proof that [ts] has aborted. *)
+    iDestruct (big_sepS_elem_of with "Hsafecp") as "Hc"; first apply Hc.
+    simpl.
+    iDestruct "Hc" as "[Habt %Hvts]".
+    rewrite /group_inv_no_log_with_cpool.
+    destruct (stm !! ts) as [st |] eqn:Hdup; last first.
+    { (* Case: Directly abort without prepare. *)
+      rewrite /group_inv_no_log_no_cpool.
+      assert (Hxfinal : cm !! ts = None).
+      { by rewrite Hcm lookup_omap Hdup. }
+      rewrite /apply_cmds foldl_snoc apply_cmds_unfold Hrsm /= Hxfinal.
+      (* Insert [(ts, true)] into the commit map. *)
+      iMod (group_commit_insert ts false with "Hcm") as "[Hcm _]".
+      { apply Hxfinal. }
+      (* Re-establish [safe_txnst]. *)
+      iDestruct (big_sepM_insert_2 _ _ ts StAborted with "[] Hsafestm") as "Hsafestm'".
+      { done. }
+      iFrame "∗ # %".
+      iPureIntro.
+      split; first done.
+      split.
+      { rewrite dom_insert_L. clear -Hdompm. set_solver. }
+      split.
+      { by rewrite Hcm omap_insert /=. }
+      split.
+      { (* Re-establish [prepared_impl_locked]. *)
+        intros t m k Hm Hk.
+        destruct (decide (t = ts)) as [-> | Hneq]; first by rewrite lookup_insert in Hm.
+        rewrite lookup_insert_ne in Hm; last done.
+        by specialize (Hpil _ _ _ Hm Hk).
+      }
+      split.
+      { (* Re-establish [locked_impl_prepared]. *)
+        intros k t Ht Hnz.
+        destruct (decide (t = ts)) as [-> | Hneq].
+        { exfalso.
+          specialize (Hlip _ _ Ht Hnz).
+          destruct Hlip as (pwrs & Hpwrs & _).
+          by rewrite Hpwrs in Hdup.
+        }
+        rewrite lookup_insert_ne; last done.
+        by specialize (Hlip _ _ Ht Hnz).
+      }
+      { rewrite lookup_insert_ne; first apply Htsnz.
+        rewrite /valid_ts in Hvts.
+        clear -Hvts. lia.
+      }
+    }
+    (* Case: Txn [ts] has prepared, aborted, or committed. *)
+    rewrite /group_inv_no_log_no_cpool.
+    (* rewrite /apply_cmds foldl_snoc apply_cmds_unfold Hrsm /= Hdup. *)
+    destruct st as [pwrs | |] eqn:Hst; first 1 last.
+    { (* Case: Committed; contradiction by obtaining a commit token. *)
+      iDestruct (big_sepM_lookup with "Hsafestm") as "Hcmt"; first apply Hdup. simpl.
+      iDestruct "Hcmt" as (wrs) "Hcmt".
+      do 2 iNamed "Htxnsys".
+      iDestruct (txn_res_lookup with "Hresm Habt") as %Habt.
+      iDestruct (txn_res_lookup with "Hresm Hcmt") as %Hcmt.
+      congruence.
+    }
+    { (* Case: Aborted; no-op. *)
+      assert (Habted : cm !! ts = Some false).
+      { by rewrite Hcm lookup_omap Hdup. }
+      rewrite /apply_cmds foldl_snoc apply_cmds_unfold Hrsm /= Habted.
+      by iFrame "∗ # %".
+    }
+    (* Case: Prepared; release the locks on tuples. *)
+    assert (Hxfinal : cm !! ts = None).
+    { by rewrite Hcm lookup_omap Hdup. }
+    rewrite /apply_cmds foldl_snoc apply_cmds_unfold Hrsm /= Hxfinal.
+    set cm' := insert _ _ cm.
+    (* Obtain proof of valid prepared input. *)
+    iDestruct (big_sepM_lookup with "Hsafestm") as "Hc"; first apply Hdup. simpl.
+    iDestruct "Hc" as "[_ Hsafepwrs]".
+    iDestruct "Hsafepwrs" as (wrs) "(Hwrs & _ & %Hvwrs & %Hne & %Hpwrs)".
+    (* Take the required keys invariants. *)
+    iDestruct (big_sepS_subseteq_acc _ _ (dom pwrs) with "Hkeys") as "[Hkeys HkeysC]".
+    { (* Prove [dom pwrs ⊆ keys_all] *)
+      transitivity (dom wrs); last done.
+      rewrite Hpwrs.
+      apply dom_filter_subseteq.
+    }
+    (* Take the required prepare timestamp from the group invariant. *)
+    iDestruct (big_sepM_dom_subseteq_difference _ _ (dom pwrs) with "Hlocks")
+      as (ptsm [Hdom Hsubseteq]) "[Hptsm HptsmO]".
+    { (* Prove [dom pwrs ⊆ dom (tpls_group gid tpls)]. *)
+      pose proof (apply_cmds_dom log _ _ Hrsm) as Hdom.
+      rewrite Hpwrs wrs_group_keys_group_dom filter_group_keys_group_dom Hdomptsm.
+      set_solver.
+    }
+    (* Expose the prepared timestamp from keys invariant. *)
+    iDestruct (keys_inv_extract_tsprep with "Hkeys") as (ptsmk) "(Hkeys & Hptsmk & %Hdomk)".
+    (* Agree on the prepare timestamps from the group and keys invariants. *)
+    iDestruct (repl_ts_big_agree with "Hptsm Hptsmk") as %->.
+    { by rewrite Hdom Hdomk. }
+    (* Reset the prepared timestamps. *)
+    iMod (repl_ts_big_update (release pwrs ptsm) with "Hptsm Hptsmk") as "[Hptsm Hptsmk]".
+    { by rewrite release_dom. }
+    (* From [prepared_impl_locked] we know keys in [dom pwrs] must be locked by [ts]. *)
+    iAssert ([∗ set] key ∈ dom pwrs, key_inv_no_tsprep γ key ts)%I
+      with "[Hkeys]" as "Hkeys".
+    { iApply (big_sepM_sepS_impl with "Hkeys"); first done.
+      iIntros (k t Ht) "!> Hkey".
+      assert (Hk : k ∈ dom pwrs).
+      { by rewrite -Hdomk elem_of_dom. }
+      specialize (Hpil _ _ _ Hdup Hk).
+      assert (Hincl : ptsm ⊆ tspreps).
+      { etrans; [apply Hsubseteq | apply map_filter_subseteq]. }
+      pose proof (lookup_weaken _ _ _ _ Ht Hincl) as Ht'.
+      rewrite Hpil in Ht'.
+      inv Ht'.
+      (* Looks like [inv Ht'] also gives [h = h'], which is useful, but is that
+      the expected behavior? *)
+      done.
+    }
+    (* Prove txn [ts] has prepared but not committed on [tpls]. *)
+    iDestruct (keys_inv_prepared (dom pwrs) with "Habt Hkeys Htxnsys") as "[Hkeys Htxnsys]".
+    (* Re-establish keys invariant w.r.t. updated prepare timestamps. *)
+    iDestruct (keys_inv_learn_abort with "Hkeys") as "Hkeys".
+    (* Put ownership of tuples back to keys invariant. *)
+    iDestruct (keys_inv_merge_tsprep (dom pwrs) with "[Hkeys] Hptsmk") as "Hkeys".
+    { by rewrite release_dom. }
+    { iApply (big_sepS_sepM_impl with "Hkeys").
+      { by rewrite release_dom. }
+      iIntros (k t Ht) "!> Hkey".
+      apply elem_of_dom_2 in Ht as Hinptsm.
+      rewrite release_dom in Hinptsm.
+      pose proof Hinptsm as Hinpwrs. rewrite Hdom in Hinpwrs.
+      pose proof (release_modified Hinpwrs Hinptsm) as Hunlocked.
+      by inv Hunlocked.
+    }
+    iDestruct ("HkeysC" with "Hkeys") as "Hkeys".
+    (* Merge ownership of prepared timestamp back to group invariant. *)
+    iDestruct (repl_ts_release_disjoint pwrs with "HptsmO") as "HptsmO".
+    { set_solver. }
+    rewrite release_difference_distr.
+    iDestruct (big_sepM_subseteq_difference_2 with "Hptsm HptsmO") as "Hptsm".
+    { by apply release_mono. }
+    rewrite release_filter_group_commute.
+    (* Insert [(ts, false)] into the commit map. *)
+    iMod (group_commit_insert ts false with "Hcm") as "[Hcm _]".
+    { apply Hxfinal. }
+    (* Re-establish [valid_prepared]. *)
+    iDestruct (big_sepM_insert_2 _ _ ts StAborted with "[] Hsafestm") as "Hsafestm'".
+    { iFrame "Habt". }
+    iFrame "∗ # %".
+    iPureIntro.
+    split; first done.
+    split.
+    { rewrite dom_insert_L. clear -Hdompm. set_solver. }
+    split.
+    { by rewrite release_dom. }
+    split.
+    { by rewrite Hcm omap_insert /=. }
+    split.
+    { (* Re-establish [prepared_impl_locked]. *)
+      intros t m k Hm Hk.
+      destruct (decide (t = ts)) as [-> | Hneq]; first by rewrite lookup_insert in Hm.
+      rewrite lookup_insert_ne in Hm; last done.
+      pose proof (Hpil _ _ _ Hm Hk) as Hkt.
+      rewrite -Hkt release_unmodified; first done.
+      apply not_elem_of_dom.
+      intros Hinpwrs.
+      specialize (Hpil _ _ _ Hdup Hinpwrs).
+      rewrite Hpil in Hkt.
+      clear -Hneq Hkt. inv Hkt.
+    }
+    split.
+    { (* Re-establish [locked_impl_prepared]. *)
+      intros k t Ht Hnz.
+      destruct (decide (k ∈ dom pwrs)) as [Hin | Hnotin].
+      { rewrite release_modified in Ht; last first.
+        { rewrite Hdomptsm.
+          rewrite /valid_wrs in Hvwrs.
+          clear -Hin Hvwrs Hpwrs.
+          assert (Hincl : dom pwrs ⊆ dom wrs).
+          { rewrite Hpwrs. apply dom_filter_subseteq. }
+          set_solver.
+        }
+        { apply Hin. }
+        clear -Hnz Ht. inv Ht.
+      }
+      rewrite release_unmodified in Ht; last first.
+      { by apply not_elem_of_dom. }
+      specialize (Hlip _ _ Ht Hnz).
+      destruct Hlip as (m & Hm & Hinm).
+      exists m.
+      destruct (decide (t = ts)) as [-> | Hneq]; last by rewrite lookup_insert_ne.
+      exfalso.
+      clear -Hm Hdup Hinm Hnotin.
+      set_solver.
+    }
+    { rewrite lookup_insert_ne; first apply Htsnz.
+      rewrite /valid_ts in Hvts.
+      clear -Hvts. lia.
+    }
+  Qed.
+
+End inv.
