src/program_proof/tulip/invariance/learn_commit.v
@@ -1,0 +1,305 @@
+From Perennial.program_proof.tulip Require Import prelude.
+From Perennial.program_proof.tulip.invariance Require Import cmd.
+
+Lemma ext_by_cmtd_inv_learn_commit repl cmtd kmod ts v :
+  kmod !! O = None ->
+  kmod !! ts = Some v ->
+  ext_by_cmtd repl cmtd kmod ts ->
+  ext_by_cmtd (last_extend ts repl ++ [v]) cmtd kmod O.
+Proof.
+  intros Hz Hts Hdiff.
+  rewrite /ext_by_cmtd Hts in Hdiff.
+  destruct Hdiff as [Hdiff _].
+  rewrite /ext_by_cmtd Hz.
+  (* by the time repl catches up cmtd, they are equal, hence using 0 here *)
+  exists O.
+  split; last done.
+  by rewrite Hdiff {2}/last_extend last_snoc /extend /= app_nil_r.
+Qed.
+
+Section inv.
+  Context `{!tulip_ghostG Σ}.
+
+  Lemma keys_inv_committed γ p ts pwrs wrs histm :
+    dom histm = dom pwrs ->
+    pwrs ⊆ wrs ->
+    is_txn_committed γ ts wrs -∗
+    ([∗ map] key ↦ hist ∈ histm, key_inv_no_repl_no_tsprep γ key hist ts) -∗
+    txnsys_inv γ p -∗
+    ([∗ map] key ↦ hist; v ∈ histm; pwrs, key_inv_cmted_no_repl_tsprep γ key hist ts v) ∗
+    txnsys_inv γ p.
+  Proof.
+    iIntros (Hdom Hwrs) "#Hcmt Hhistm Htxnsys".
+    iApply (big_sepM_sepM2_impl_res with "Hhistm Htxnsys"); first done.
+    iIntros "!>" (k h v Htpl Hv) "Hkey Htxnsys".
+    do 2 iNamed "Htxnsys".
+    iDestruct (txn_res_lookup with "Hresm Hcmt") as %Hresm.
+    do 2 iNamed "Hkey".
+    iDestruct (cmtd_kmod_vslice_agree with "Hkmodcs Hkmodc") as %Hkmodc.
+    { apply Hall. }
+    assert (Hwrsv : wrs !! k = Some v); first by eapply lookup_weaken.
+    assert (Hkmodcv : kmodc !! ts = Some v).
+    { subst kmodc. by eapply vslice_resm_to_tmods_committed_present. }
+    iAssert (txnsys_inv γ p)%I with "[-Hkmodl Hkmodc Hdbv Hlnrz Hcmtd]" as "Htxnsys".
+    { iFrame "∗ # %". }
+    iFrame "∗ # %".
+  Qed.
+
+  Lemma txnsys_inv_has_prepared γ p gid ts wrs :
+    gid ∈ ptgroups (dom wrs) ->
+    is_txn_committed γ ts wrs -∗
+    txnsys_inv γ p -∗
+    is_group_prepared γ gid ts.
+  Proof.
+    iIntros (Hptg) "Hres Htxnsys".
+    do 2 iNamed "Htxnsys".
+    iDestruct (txn_res_lookup with "Hresm Hres") as %Hr.
+    iDestruct (big_sepM_lookup with "Hvr") as "Hr"; first by apply Hr.
+    iDestruct "Hr" as "[_ Hpreps]".
+    iDestruct (big_sepS_elem_of with "Hpreps") as "Hprep"; first apply Hptg.
+    iFrame "#".
+  Qed.
+
+  Lemma key_inv_learn_commit {γ ts wrs hists} k h v h' :
+    hists !! k = Some h ->
+    wrs !! k = Some v ->
+    multiwrite ts wrs hists !! k = Some h' ->
+    key_inv_cmted_no_repl_tsprep γ k h ts v -∗
+    key_inv_no_repl_no_tsprep γ k h' O.
+  Proof.
+    iIntros (Hh Hv Hh') "Hkey".
+    do 3 iNamed "Hkey".
+    iFrame "∗ # %".
+    iPureIntro.
+    rewrite lookup_merge Hv Hh /= in Hh'.
+    inv Hh'.
+    split.
+    { by destruct (last_extend _ _). }
+    by apply ext_by_cmtd_inv_learn_commit.
+  Qed.
+
+  Lemma keys_inv_learn_commit {γ ts wrs hists} :
+    ([∗ map] key ↦ hist; v ∈ hists; wrs, key_inv_cmted_no_repl_tsprep γ key hist ts v) -∗
+    ([∗ map] key ↦ hist ∈ multiwrite ts wrs hists, key_inv_no_repl_no_tsprep γ key hist O).
+  Proof.
+    iIntros "Hkeys".
+    iApply (big_sepM2_sepM_impl with "Hkeys").
+    { apply multiwrite_dom. }
+    iIntros "!>" (k h v h' Hh Hv Hh') "Hkey".
+    by iApply (key_inv_learn_commit with "Hkey").
+  Qed.
+
+  Lemma group_inv_learn_commit γ p gid log cpool ts pwrs :
+    cpool_subsume_log cpool (log ++ [CmdCommit ts pwrs]) ->
+    txnsys_inv γ p -∗
+    ([∗ set] key ∈ keys_all, key_inv γ key) -∗
+    group_inv_no_log_with_cpool γ gid log cpool ==∗
+    txnsys_inv γ p ∗
+    ([∗ set] key ∈ keys_all, key_inv γ key) ∗
+    group_inv_no_log_with_cpool γ gid (log ++ [CmdCommit ts pwrs]) cpool.
+  Proof.
+    iIntros (Hsubsume) "Htxnsys Hkeys Hgroup".
+    rewrite /cpool_subsume_log Forall_app Forall_singleton in Hsubsume.
+    destruct Hsubsume as [Hsubsume Hc].
+    do 2 iNamed "Hgroup".
+    (* Obtain proof that [ts] has committed. *)
+    iDestruct (big_sepS_elem_of with "Hsafecp") as "Hc"; first apply Hc.
+    simpl.
+    iDestruct "Hc" as (wrs) "(Hcmt & Hwrs & %Hpwrs & %Hgid)".
+    rewrite /group_inv_no_log_with_cpool.
+    destruct (stm !! ts) as [st |] eqn:Hdup; last first.
+    { (* Case: Empty state; contradiction---no prepare before commit. *) 
+      iDestruct (txnsys_inv_has_prepared with "Hcmt Htxnsys") as "#Hst"; first apply Hgid.
+      assert (Hpm : pm !! ts = None).
+      { rewrite -not_elem_of_dom. rewrite -not_elem_of_dom in Hdup. set_solver. }
+      iDestruct (group_prep_lookup with "Hpm Hst") as %Hlookup.
+      congruence.
+    }
+    (* Case: Transaction prepared, aborted, or committed. *)
+    destruct st as [pwrs' | |] eqn:Hst; last first.
+    { (* Case: [StAborted]; contradiction. *)
+      iDestruct (big_sepM_lookup with "Hsafestm") as "#Habt"; first apply Hdup.
+      do 2 iNamed "Htxnsys".
+      iDestruct (txn_res_lookup with "Hresm Hcmt") as "%Hcmt".
+      iDestruct (txn_res_lookup with "Hresm Habt") as "%Habt".
+      congruence.
+    }
+    { (* Case: [StCommitted]; no-op. *)
+      iFrame "∗ # %".
+      iPureIntro.
+      assert (Hcmted : cm !! ts = Some true).
+      { by rewrite Hcm lookup_omap Hdup. }
+      by rewrite /apply_cmds foldl_snoc apply_cmds_unfold Hrsm /= Hcmted.
+    }
+    (* Case: [StPrepared wrs] *)
+    assert (Hxfinal : cm !! ts = None).
+    { by rewrite Hcm lookup_omap Hdup. }
+    rewrite /group_inv_no_log_no_cpool.
+    rewrite /apply_cmds foldl_snoc apply_cmds_unfold Hrsm /= Hxfinal.
+    set cm' := insert _ _ cm.
+    set histm' := multiwrite _ _ _.
+    (* Obtain proof of valid prepared input. *)
+    iDestruct (big_sepM_lookup with "Hsafestm") as "Hc"; first apply Hdup. simpl.
+    iDestruct "Hc" as "[_ Hsafepwrs]".
+    iDestruct "Hsafepwrs" as (wrs') "(Hwrs' & %Hvts & %Hvwrs & %Hne & %Hpwrs')".
+    iDestruct (txn_wrs_agree with "Hwrs Hwrs'") as %->.
+    rewrite -Hpwrs in Hpwrs'. subst pwrs'.
+    (* Take the required keys invariants. *)
+    iDestruct (big_sepS_subseteq_acc _ _ (dom pwrs) with "Hkeys") as "[Hkeys HkeysC]".
+    { (* Prove [dom pwrs ⊆ keys_all] *)
+      transitivity (dom wrs); last done.
+      rewrite Hpwrs.
+      apply dom_filter_subseteq.
+    }
+    (* Take the required history and prepare timestamp from the group invariant. *)
+    iDestruct (big_sepM_dom_subseteq_difference _ _ (dom pwrs) with "Hhists")
+      as (histm [Hdomhistmg Hinclhistmg]) "[Hhistm HhistmO]".
+    { (* Prove [dom pwrs ⊆ dom (tpls_group gid tpls)]. *)
+      pose proof (apply_cmds_dom log _ _ Hrsm) as Hdom.
+      rewrite Hpwrs wrs_group_keys_group_dom filter_group_keys_group_dom Hdom.
+      clear -Hvwrs. set_solver.
+    }
+    iDestruct (big_sepM_dom_subseteq_difference _ _ (dom pwrs) with "Hlocks")
+      as (ptsm [Hdomptsmg Hinclptsmg]) "[Hptsm HptsmO]".
+    { (* Prove [dom pwrs ⊆ dom (tpls_group gid tpls)]. *)
+      pose proof (apply_cmds_dom log _ _ Hrsm) as Hdom.
+      rewrite Hpwrs wrs_group_keys_group_dom filter_group_keys_group_dom Hdomptsm.
+      clear -Hvwrs. set_solver.
+    }
+    (* Extract the replicated history and prepared timestamp from keys invariant. *)
+    iDestruct (keys_inv_extract_repl_pts with "Hkeys")
+      as (histmk ptsmk) "(Hkeys & Hhistmk & Hptsmk & %Hdomhistmk)".
+    iDestruct (big_sepM2_dom with "Hkeys") as %Hdomptsmk.
+    symmetry in Hdomptsmk. rewrite Hdomhistmk in Hdomptsmk.
+    (* Agree on history map from the group and keys invariants. *)
+    iDestruct (repl_hist_big_agree with "Hhistm Hhistmk") as %->.
+    { by rewrite Hdomhistmg Hdomhistmk. }
+    (* Extending the replicated history. *)
+    iMod (repl_hist_big_update (multiwrite ts pwrs histm) with "Hhistm Hhistmk")
+      as "[Hhistm Hhistmk]".
+    { rewrite map_Forall2_forall.
+      split; last by rewrite multiwrite_dom.
+      intros k h1 h2 Hh1 Hh2.
+      apply elem_of_dom_2 in Hh1 as Hv.
+      rewrite Hdomhistmk elem_of_dom in Hv.
+      destruct Hv as [v Hv].
+      rewrite (multiwrite_modified Hv Hh1) in Hh2.
+      inv Hh2.
+      apply prefix_app_r, last_extend_prefix.
+    }
+    (* Agree on history map from the group and keys invariants. *)
+    iDestruct (repl_ts_big_agree with "Hptsm Hptsmk") as %->.
+    { by rewrite Hdomptsmg Hdomptsmk. }
+    (* Reset the prepared timestamp. *)
+    iMod (repl_ts_big_update (release pwrs ptsm) with "Hptsm Hptsmk") as "[Hptsm Hptsmk]".
+    { by rewrite release_dom. }
+    (* From [prepared_impl_locked] we know keys in [dom pwrs] must be locked by [ts]. *)
+    iAssert ([∗ map] key ↦ hist ∈ histm, key_inv_no_repl_no_tsprep γ key hist ts)%I
+      with "[Hkeys]" as "Hkeys".
+    { iApply (big_sepM2_sepM_impl with "Hkeys"); first done.
+      iIntros (k h t h' Hh Ht Hh') "!> Hkey".
+      assert (Hk : k ∈ dom pwrs).
+      { by rewrite -Hdomhistmg elem_of_dom. }
+      specialize (Hpil _ _ _ Hdup Hk).
+      assert (Hincl : ptsm ⊆ tspreps).
+      { etrans; [apply Hinclptsmg | apply map_filter_subseteq]. }
+      pose proof (lookup_weaken _ _ _ _ Ht Hincl) as Ht'.
+      rewrite Hpil in Ht'.
+      inv Ht'.
+      (* Looks like [inv Ht'] also gives [h = h'], which is useful, but is that
+      the expected behavior? *)
+      done.
+    }
+    (* Prove txn [ts] has committed on [tpls]. *)
+    iDestruct (keys_inv_committed with "Hcmt Hkeys Htxnsys") as "[Hkeys Htxnsys]".
+    { apply Hdomhistmg. }
+    { rewrite Hpwrs. apply map_filter_subseteq. }
+    (* Re-establish keys invariant w.r.t. updated tuples. *)
+    iDestruct (keys_inv_learn_commit with "Hkeys") as "Hkeys".
+    (* Put ownership of tuples back to keys invariant. *)
+    iDestruct (keys_inv_merge_repl_pts (dom pwrs) with "[Hkeys] Hhistmk Hptsmk") as "Hkeys".
+    { by rewrite multiwrite_dom. }
+    { iApply (big_sepM_sepM2_impl with "Hkeys").
+      { by rewrite release_dom multiwrite_dom Hdomhistmg Hdomptsmg. }
+      iIntros (k h t Hh Ht) "!> Hkey".
+      apply elem_of_dom_2 in Hh as Hinpwrs.
+      rewrite multiwrite_dom Hdomhistmg in Hinpwrs.
+      pose proof Hinpwrs as Hinptsm. rewrite -Hdomptsmg in Hinptsm.
+      pose proof (release_modified Hinpwrs Hinptsm) as Hunlocked.
+      by inv Hunlocked.
+    }
+    iDestruct ("HkeysC" with "Hkeys") as "Hkeys".
+    (* Merge ownership of replicated history back to group invariant. *)
+    iDestruct (repl_hist_multiwrite_disjoint ts pwrs with "HhistmO") as "HhistmO".
+    { set_solver. }
+    rewrite multiwrite_difference_distr.
+    iDestruct (big_sepM_subseteq_difference_2 with "Hhistm HhistmO") as "Hhistm".
+    { by apply multiwrite_mono. }
+    rewrite multiwrite_filter_group_commute.
+    (* Merge ownership of prepared timestamp back to group invariant. *)
+    iDestruct (repl_ts_release_disjoint pwrs with "HptsmO") as "HptsmO".
+    { set_solver. }
+    rewrite release_difference_distr.
+    iDestruct (big_sepM_subseteq_difference_2 with "Hptsm HptsmO") as "Hptsm".
+    { by apply release_mono. }
+    rewrite release_filter_group_commute.
+    (* Insert [(ts, true)] into the commit map. *)
+    iMod (group_commit_insert ts true with "Hcm") as "[Hcm _]".
+    { apply Hxfinal. }
+    (* Re-establish [safe_txnst]. *)
+    iDestruct (big_sepM_insert_2 _ _ ts (StCommitted) with "[] Hsafestm") as "Hsafestm'".
+    { iFrame "Hcmt". }
+    iFrame "∗ # %".
+    iPureIntro.
+    split; first done.
+    split.
+    { rewrite dom_insert_L. clear -Hdompm. set_solver. }
+    split.
+    { by rewrite release_dom. }
+    split.
+    { by rewrite Hcm omap_insert /=. }
+    split.
+    { (* Re-establish [prepared_impl_locked]. *)
+      intros t m k Hm Hk.
+      destruct (decide (t = ts)) as [-> | Hneq]; first by rewrite lookup_insert in Hm.
+      rewrite lookup_insert_ne in Hm; last done.
+      pose proof (Hpil _ _ _ Hm Hk) as Hkt.
+      rewrite -Hkt release_unmodified; first done.
+      apply not_elem_of_dom.
+      intros Hinpwrs.
+      specialize (Hpil _ _ _ Hdup Hinpwrs).
+      rewrite Hpil in Hkt.
+      clear -Hneq Hkt. inv Hkt.
+    }
+    split.
+    { (* Re-establish [locked_impl_prepared]. *)
+      intros k t Ht Hnz.
+      destruct (decide (k ∈ dom pwrs)) as [Hin | Hnotin].
+      { rewrite release_modified in Ht; last first.
+        { rewrite Hdomptsm.
+          rewrite /valid_wrs in Hvwrs.
+          clear -Hin Hvwrs Hpwrs.
+          assert (Hincl : dom pwrs ⊆ dom wrs).
+          { rewrite Hpwrs. apply dom_filter_subseteq. }
+          set_solver.
+        }
+        { apply Hin. }
+        clear -Hnz Ht. inv Ht.
+      }
+      rewrite release_unmodified in Ht; last first.
+      { by apply not_elem_of_dom. }
+      specialize (Hlip _ _ Ht Hnz).
+      destruct Hlip as (m & Hm & Hinm).
+      exists m.
+      destruct (decide (t = ts)) as [-> | Hneq]; last by rewrite lookup_insert_ne.
+      exfalso.
+      clear -Hm Hdup Hinm Hnotin.
+      set_solver.
+    }
+    { rewrite lookup_insert_ne; first apply Htsnz.
+      rewrite /valid_ts in Hvts.
+      clear -Hvts. lia.
+    }
+  Qed.
+
+End inv.
